SystemF2Effect: work on Preservation
Ignore-this: cf4d1723f20ae92f76e266c721fc24c3

darcs-hash:20121230000312-08f32-2569d3b6b730359b066fba3f9ac19732925af377

devel/Iron/Language/SystemF2Effect/Store.v
@@ -1,4 +1,5 @@
 
+Require Import Iron.Language.SystemF2Effect.Ty.
 Require Import Iron.Language.SystemF2Effect.TyJudge.
 Require Import Iron.Language.SystemF2Effect.VaExpBase.
 
@@ -26,8 +27,20 @@ Hint Unfold STORET.
 (*******************************************************************)
 (* Well formed store. *)
 Definition WfS (se: stenv) (ss: list val)
- := STOREM se ss
+ := Forall closedT se
+ /\ STOREM se ss
  /\ STORET se ss.
+Hint Unfold WfS.
 
 
-
+(********************************************************************)
+(* When we extend the store and store typing with a new binding, 
+   then the resulting store is still well formed. *)
+Lemma store_extended_wellformed
+ :  forall se ss v t
+ ,  WfS    se ss
+ -> TYPEV  nil nil se v t
+ -> WfS    (t <: se) (v <: ss).
+Proof.
+ admit.
+Qed.
