devel/Iron/Language/SystemF2Effect/Preservation.v
@@ -1,0 +1,78 @@
+
+Require Import Iron.Language.SystemF2Effect.Step.
+Require Import Iron.Language.SystemF2Effect.TyJudge.
+Require Import Iron.Language.SystemF2Effect.TyEnv.
+Require Import Iron.Language.SystemF2Effect.KiJudge.
+Require Import Iron.Language.SystemF2Effect.SubstValExp.
+Require Import Iron.Language.SystemF2Effect.SubstTypeExp.
+Require Import Iron.Language.SystemF2Effect.Store.
+
+
+(* When a well typed expression transitions to the next state
+   then its type is preserved. *)
+Theorem preservation
+ :  forall se s x s' x' t e
+ ,  WfS se s
+ -> TYPEX nil nil se x  t e
+ -> STEP s x s' x'
+ -> (exists se' e'
+            ,  extends se' se
+            /\ WfS  se' s'
+            /\ SubsT e e'
+            /\ TYPEX nil nil se' x' t e').
+Proof.
+ intros se s x s' x' t e HH HT HS. gen t e.
+ induction HS; intros; inverts_type; rip.
+
+ Case "EsLet".
+  spec IHHS t e1. rip.
+  shift se'.
+  destruct H as [e1'].
+  exists (TSum e1' e2).
+  inverts HH.
+  rip.
+   inverts H; burn.
+   inverts H; burn.
+   inverts H; burn.
+   
+ Case "EsLetSubst".
+  exists se. exists e2.
+  rip.
+  burn.
+  eapply subst_val_exp; eauto.
+
+ Case "EsAppSubst".
+  exists se. exists e.
+  rip.
+  eapply subst_val_exp; eauto.
+
+ Case "EsLAMSubst".
+  exists se. exists (TBot KEffect).
+  rip.
+  assert (TYPEX nil (substTE 0 t2 nil) (substTE 0 t2 se)
+                (substTX 0 t2 x12) 
+                (substTT 0 t2 t12)     (substTT 0 t2 (TBot KEffect))).
+   eapply subst_type_exp; eauto.
+
+   inverts HH. rip. eauto.
+   rrwrite (liftTE 0 nil = nil).
+   rrwrite (liftTE 0 se  = se). 
+   auto.
+
+   inverts HH. rip. eauto.
+   rrwrite (substTE 0 t2 nil = nil).
+   rrwrite (substTE 0 t2 se  = se).
+   norm.
+
+ Case "EsAlloc".
+  exists (t2 <: se).
+  exists (tAlloc t1).
+  rip.
+
+  (* New store is well formed under the extended store typing. *)
+  eapply store_extended_wellformed; eauto.
+  
+  
+
+
+
