devel/Iron/Language/SystemF2Effect/Ty.v
@@ -3,3 +3,4 @@ Require Export Iron.Language.SystemF2Effect.TyCon.
 Require Export Iron.Language.SystemF2Effect.TyExp.
 Require Export Iron.Language.SystemF2Effect.TyLift.
 Require Export Iron.Language.SystemF2Effect.TySubst.
+Require Export Iron.Language.SystemF2Effect.TyWfT.
